More config marshal proof; need to change another forSlice to normal for

src/program_proof/simplepb/config_marshal_proof.v
@@ -8,7 +8,7 @@ Section Config.
 Definition C := list u64.
 
 Definition has_encoding (encoded:list u8) (args:C) : Prop :=
-  encoded u64_le (length args) ++ concat (u64_le <$> args).
+  encoded = u64_le (length args) ++ concat (u64_le <$> args).
 
 Context `{!heapGS Σ}.
 
@@ -51,26 +51,120 @@ Proof.
 
   replace (conf_sl.(Slice.sz)) with (U64 (length conf)) by word.
   set (P:=(λ (i:u64),
-      "Henc" ∷ is_slice enc_sl byteT 1 ((u64_le (length conf)) ++ concat (u64_le <$> (take (int.nat i) conf))) ∗
-      "Henc" ∷ True
+      ∃ enc_sl,
+      "Henc_sl" ∷ is_slice enc_sl byteT 1 ((u64_le (length conf)) ++ concat (u64_le <$> (take (int.nat i) conf))) ∗
+      "Henc" ∷ enc ↦[slice.T byteT] (slice_val enc_sl)
     )%I)
   .
-  wp_apply (wp_forSlice P with "[] [$Hconf]").
+  wp_apply (wp_forSlice P with "[] [$Hconf Henc Henc_sl]").
   {
     iIntros (i srv).
     clear Φ.
-    iIntros (Φ) "!# (HP & %Hi & %Hlookup) HΦ".
-Admitted.
+    iIntros (Φ) "!# (HP & %Hi_bound & %Hlookup) HΦ".
+    iNamed "HP".
+
+    wp_pures.
+    wp_load.
+    wp_apply (wp_WriteInt with "Henc_sl").
+    iIntros (enc_sl') "Henc_sl".
+    wp_store.
+    iModIntro.
+    iApply "HΦ".
+    unfold P.
+    iExists _; iFrame "Henc".
+    iApply to_named.
+    iExactEq "Henc_sl".
+    f_equal.
+
+    (* Start pure proof *)
+    (* prove that appending the encoded next entry results in a concatenation of
+       the first (i+1) entries *)
+    rewrite -app_assoc.
+    f_equal.
+    replace (u64_le srv) with (concat (u64_le <$> [srv])) by done.
+    rewrite -concat_app.
+    rewrite -fmap_app.
+    replace (int.nat (word.add i 1)) with (int.nat i + 1)%nat by word.
+    f_equal.
+    f_equal.
+    (* TODO: list_solver *)
+    rewrite take_more; last word.
+    f_equal.
+    apply list_eq.
+    intros.
+    destruct i0.
+    {
+      simpl.
+      rewrite lookup_take; last lia.
+      rewrite lookup_drop.
+      rewrite -Hlookup.
+      f_equal.
+      word.
+    }
+    {
+      simpl.
+      rewrite lookup_nil.
+      rewrite lookup_take_ge; last word.
+      done.
+    }
+    (* End pure proof *)
+  }
+  {
+    unfold P.
+    iExists _; iFrame.
+  }
+  iIntros "[HP Hconf_sl]".
+  iNamed "HP".
+  wp_pures.
+  wp_load.
+  iApply "HΦ".
+  iModIntro.
+  iFrame.
+  rewrite -Hsz.
+  iPureIntro.
+  unfold has_encoding.
+  rewrite firstn_all.
+  done.
+Qed.
 
 Lemma wp_Decode enc enc_sl (conf:C) :
   {{{
         ⌜has_encoding enc conf⌝ ∗
-        is_slice enc_sl byteT 1 enc
+        is_slice_small enc_sl byteT 1 enc
   }}}
     config.DecodeConfig (slice_val enc_sl)
   {{{
         conf_sl, RET (slice_val conf_sl); own conf_sl conf
   }}}.
+Proof.
+  iIntros (Φ) "[%Henc Henc_sl] HΦ".
+  wp_call.
+  wp_apply (wp_ref_to).
+  { done. }
+  iIntros (enc_ptr) "Henc".
+  wp_pures.
+  wp_apply (wp_ref_of_zero).
+  { done. }
+  iIntros (configLen_ptr) "HconfigLen".
+  wp_pures.
+  wp_load.
+  rewrite Henc.
+  wp_apply (wp_ReadInt with "[$Henc_sl]").
+  iIntros (enc_sl') "Henc_sl".
+  wp_store.
+  wp_store.
+
+  wp_load.
+  wp_apply (wp_NewSlice).
+  iIntros (conf_sl) "Hconf_sl".
+  wp_pures.
+
+  set (P:=(λ (i:u64),
+      ∃ enc_sl,
+      "Henc_sl" ∷ is_slice enc_sl byteT 1 (concat (u64_le <$> (drop (int.nat i) conf))) ∗
+      "Henc" ∷ enc_ptr ↦[slice.T byteT] (slice_val enc_sl)
+    )%I)
+  .
 Admitted.
 
 End Config.
